ccc26x86/Asm_event.v
@@ -8,25 +8,25 @@ Require Import compcert.common.Memory.
 Require Import compcert.common.Events.
 Require Import compcert.common.Globalenvs.
 Require Import compcert.common.Smallstep.
-Require Import VST.ccc26x86.Locations.
-(*Require Import Stacklayout.*)
-Require Import VST.ccc26x86.Conventions.
+Require Import compcert.backend.Locations.
+Require Import compcert.x86.Stacklayout.
+Require Import compcert.backend.Conventions.
 
-Require Import VST.ccc26x86.Asm.
+Require Import compcert.x86.Asm.
 (*LENB: In CompComp, we used a modified Asm.v, called Asm.comp.v*)
 
 Require Import VST.sepcomp.mem_lemmas.
-Require Import VST.sepcomp.semantics.
+Require Import VST.concurrency.core_semantics.
 Require Import VST.sepcomp.semantics_lemmas.
 Require Import VST.sepcomp.val_casted.
 Require Import VST.ccc26x86.BuiltinEffects.
-Require Import VST.ccc26x86.load_frame.
+(*Require Import VST.ccc26x86.load_frame.*)
 Require Import VST.sepcomp.event_semantics.
 Require Import VST.ccc26x86.Asm_coop.
 
 Require Import List. Import ListNotations.
 (*
-Notation SP := ESP (only parsing).
+Notation SP := RSP (only parsing).
 
 Notation "a # b" := (a b) (at level 1, only parsing).
 Notation "a # b <- c" := (Pregmap.set b c a) (at level 1, b at next level).
@@ -45,149 +45,160 @@ Definition drf_instr (ge:genv) (c: code) (i: instruction) (rs: regset) (m: mem)
            : option (list mem_event)  :=
   match i with
   | Pfstps_m a => match eval_addrmode ge a rs with
-                    Vptr b ofs => Some [Write b (Int.unsigned ofs) (encode_val Mfloat32 (rs ST0))]
+                    Vptr b ofs => Some [Write b (Ptrofs.unsigned ofs) (encode_val Mfloat32 (rs ST0))]
                   | _ => None
                  end
   | Pfstpl_m a => match eval_addrmode ge a rs with
-                    Vptr b ofs => Some [Write b (Int.unsigned ofs) (encode_val Mfloat64 (rs ST0))]
+                    Vptr b ofs => Some [Write b (Ptrofs.unsigned ofs) (encode_val Mfloat64 (rs ST0))]
                   | _ => None
                  end
   | Pmovss_mf a r1 => match eval_addrmode ge a rs with
-                    Vptr b ofs => Some [Write b (Int.unsigned ofs) (encode_val Mfloat32 (rs r1))]
+                    Vptr b ofs => Some [Write b (Ptrofs.unsigned ofs) (encode_val Mfloat32 (rs r1))]
                   | _ => None
                  end
-  | Pmov_mr a r1 => match eval_addrmode ge a rs with
-                    Vptr b ofs => Some [Write b (Int.unsigned ofs) (encode_val Mint32 (rs r1))]
+  | Pmovl_mr a r1 => match eval_addrmode ge a rs with
+                    Vptr b ofs => Some [Write b (Ptrofs.unsigned ofs) (encode_val Mint32 (rs r1))]
+                  | _ => None
+                 end
+  | Pmovq_mr a r1 => match eval_addrmode ge a rs with
+                    Vptr b ofs => Some [Write b (Ptrofs.unsigned ofs) (encode_val Mint64 (rs r1))]
                   | _ => None
                  end
   | Pmov_mr_a a r1 => match eval_addrmode ge a rs with
-                    Vptr b ofs => Some [Write b (Int.unsigned ofs) (encode_val Many32 (rs r1))]
+                    Vptr b ofs => Some [Write b (Ptrofs.unsigned ofs) (encode_val Many32 (rs r1))]
                   | _ => None
                  end
   | Pmovsd_mf a r1 => match eval_addrmode ge a rs with
-                    Vptr b ofs => Some [Write b (Int.unsigned ofs) (encode_val Mfloat64 (rs r1))]
+                    Vptr b ofs => Some [Write b (Ptrofs.unsigned ofs) (encode_val Mfloat64 (rs r1))]
                   | _ => None
                  end
   | Pmovsd_mf_a a r1 => match eval_addrmode ge a rs with
-                    Vptr b ofs => Some [Write b (Int.unsigned ofs)  (encode_val Many64 (rs r1))]
+                    Vptr b ofs => Some [Write b (Ptrofs.unsigned ofs)  (encode_val Many64 (rs r1))]
                   | _ => None
                  end
   | Pmovb_mr a r1 => match eval_addrmode ge a rs with
-                    Vptr b ofs => Some [Write b (Int.unsigned ofs) (encode_val Mint8unsigned (rs r1))]
+                    Vptr b ofs => Some [Write b (Ptrofs.unsigned ofs) (encode_val Mint8unsigned (rs r1))]
                   | _ => None
                  end
   | Pmovw_mr a r1 => match eval_addrmode ge a rs with
-                    Vptr b ofs => Some [Write b (Int.unsigned ofs) (encode_val Mint16unsigned (rs r1))]
+                    Vptr b ofs => Some [Write b (Ptrofs.unsigned ofs) (encode_val Mint16unsigned (rs r1))]
                   | _ => None
                  end
 
-  | Pmov_rm rd a => match eval_addrmode ge a rs with
-                    Vptr b ofs => match Mem.loadbytes m b (Int.unsigned ofs) (size_chunk Mint32) with
-                                    Some bytes => Some [Read b (Int.unsigned ofs) (size_chunk Mint32) bytes]
+  | Pmovl_rm rd a => match eval_addrmode ge a rs with
+                    Vptr b ofs => match Mem.loadbytes m b (Ptrofs.unsigned ofs) (size_chunk Mint32) with
+                                    Some bytes => Some [Read b (Ptrofs.unsigned ofs) (size_chunk Mint32) bytes]
+                                  | None => None
+                                  end
+                  | _ => None
+                 end
+  | Pmovq_rm rd a => match eval_addrmode ge a rs with
+                    Vptr b ofs => match Mem.loadbytes m b (Ptrofs.unsigned ofs) (size_chunk Mint64) with
+                                    Some bytes => Some [Read b (Ptrofs.unsigned ofs) (size_chunk Mint64) bytes]
                                   | None => None
                                   end
                   | _ => None
                  end
   | Pmovsd_fm rd a => match eval_addrmode ge a rs with
-                    Vptr b ofs => match Mem.loadbytes m b (Int.unsigned ofs) (size_chunk Mfloat64) with
-                                    Some bytes => Some [Read b (Int.unsigned ofs) (size_chunk Mfloat64) bytes]
+                    Vptr b ofs => match Mem.loadbytes m b (Ptrofs.unsigned ofs) (size_chunk Mfloat64) with
+                                    Some bytes => Some [Read b (Ptrofs.unsigned ofs) (size_chunk Mfloat64) bytes]
                                   | None => None
                                   end
                   | _ => None
                  end
   | Pmovss_fm rd a => match eval_addrmode ge a rs with
-                    Vptr b ofs => match Mem.loadbytes m b (Int.unsigned ofs) (size_chunk Mfloat32) with
-                                    Some bytes => Some [Read b (Int.unsigned ofs) (size_chunk Mfloat32) bytes]
+                    Vptr b ofs => match Mem.loadbytes m b (Ptrofs.unsigned ofs) (size_chunk Mfloat32) with
+                                    Some bytes => Some [Read b (Ptrofs.unsigned ofs) (size_chunk Mfloat32) bytes]
                                   | None => None
                                   end
                   | _ => None
                   end
   | Pfldl_m a => match eval_addrmode ge a rs with
-                    Vptr b ofs => match Mem.loadbytes m b (Int.unsigned ofs) (size_chunk Mfloat64) with
-                                    Some bytes => Some [Read b (Int.unsigned ofs) (size_chunk Mfloat64) bytes]
+                    Vptr b ofs => match Mem.loadbytes m b (Ptrofs.unsigned ofs) (size_chunk Mfloat64) with
+                                    Some bytes => Some [Read b (Ptrofs.unsigned ofs) (size_chunk Mfloat64) bytes]
                                   | None => None
                                   end
                   | _ => None
                   end
   | Pflds_m a => match eval_addrmode ge a rs with
-                    Vptr b ofs => match Mem.loadbytes m b (Int.unsigned ofs) (size_chunk Mfloat32) with
-                                    Some bytes => Some [Read b (Int.unsigned ofs) (size_chunk Mfloat32) bytes]
+                    Vptr b ofs => match Mem.loadbytes m b (Ptrofs.unsigned ofs) (size_chunk Mfloat32) with
+                                    Some bytes => Some [Read b (Ptrofs.unsigned ofs) (size_chunk Mfloat32) bytes]
                                   | None => None
                                   end
                   | _ => None
                   end
   | Pmovzb_rm rd a => match eval_addrmode ge a rs with
-                    Vptr b ofs => match Mem.loadbytes m b (Int.unsigned ofs) (size_chunk Mint8unsigned) with
-                                    Some bytes => Some [Read b (Int.unsigned ofs) (size_chunk Mint8unsigned) bytes]
+                    Vptr b ofs => match Mem.loadbytes m b (Ptrofs.unsigned ofs) (size_chunk Mint8unsigned) with
+                                    Some bytes => Some [Read b (Ptrofs.unsigned ofs) (size_chunk Mint8unsigned) bytes]
                                   | None => None
                                   end
                   | _ => None
                   end
   | Pmovsb_rm rd a => match eval_addrmode ge a rs with
-                    Vptr b ofs => match Mem.loadbytes m b (Int.unsigned ofs) (size_chunk Mint8signed) with
-                                    Some bytes => Some [Read b (Int.unsigned ofs) (size_chunk Mint8signed) bytes]
+                    Vptr b ofs => match Mem.loadbytes m b (Ptrofs.unsigned ofs) (size_chunk Mint8signed) with
+                                    Some bytes => Some [Read b (Ptrofs.unsigned ofs) (size_chunk Mint8signed) bytes]
                                   | None => None
                                   end
                   | _ => None
                   end
   | Pmovzw_rm rd a => match eval_addrmode ge a rs with
-                    Vptr b ofs => match Mem.loadbytes m b (Int.unsigned ofs) (size_chunk Mint16unsigned) with
-                                    Some bytes => Some [Read b (Int.unsigned ofs) (size_chunk Mint16unsigned) bytes]
+                    Vptr b ofs => match Mem.loadbytes m b (Ptrofs.unsigned ofs) (size_chunk Mint16unsigned) with
+                                    Some bytes => Some [Read b (Ptrofs.unsigned ofs) (size_chunk Mint16unsigned) bytes]
                                   | None => None
                                   end
                   | _ => None
                   end
   | Pmovsw_rm rd a => match eval_addrmode ge a rs with
-                    Vptr b ofs => match Mem.loadbytes m b (Int.unsigned ofs) (size_chunk Mint16signed) with
-                                    Some bytes => Some [Read b (Int.unsigned ofs) (size_chunk Mint16signed) bytes]
+                    Vptr b ofs => match Mem.loadbytes m b (Ptrofs.unsigned ofs) (size_chunk Mint16signed) with
+                                    Some bytes => Some [Read b (Ptrofs.unsigned ofs) (size_chunk Mint16signed) bytes]
                                   | None => None
                                   end
                   | _ => None
                   end
   | Pmov_rm_a rd a => match eval_addrmode ge a rs with
-                    Vptr b ofs => match Mem.loadbytes m b (Int.unsigned ofs) (size_chunk Many32) with
-                                    Some bytes => Some [Read b (Int.unsigned ofs) (size_chunk Many32) bytes]
+                    Vptr b ofs => match Mem.loadbytes m b (Ptrofs.unsigned ofs) (size_chunk Many32) with
+                                    Some bytes => Some [Read b (Ptrofs.unsigned ofs) (size_chunk Many32) bytes]
                                   | None => None
                                   end
                   | _ => None
                   end
   | Pmovsd_fm_a rd a => match eval_addrmode ge a rs with
-                    Vptr b ofs => match Mem.loadbytes m b (Int.unsigned ofs) (size_chunk Many64) with
-                                    Some bytes => Some [Read b (Int.unsigned ofs) (size_chunk Many64) bytes]
+                    Vptr b ofs => match Mem.loadbytes m b (Ptrofs.unsigned ofs) (size_chunk Many64) with
+                                    Some bytes => Some [Read b (Ptrofs.unsigned ofs) (size_chunk Many64) bytes]
                                   | None => None
                                   end
                   | _ => None
                   end
   | Pallocframe sz ofs_ra ofs_link =>
       let (m1, stk) := Mem.alloc m 0 sz in
-      let sp := Vptr stk Int.zero in
-      match Mem.storev Mint32 m1 (Val.add sp (Vint ofs_link)) rs#ESP with
+      let sp := Vptr stk Ptrofs.zero in
+      match Mem.storev Mptr m1 (Val.offset_ptr sp ofs_link) rs#RSP with
       | None => None
       | Some m2 =>
-          match Mem.storev Mint32 m2 (Val.add sp (Vint ofs_ra)) rs#RA with
+          match Mem.storev Mptr m2 (Val.offset_ptr sp ofs_ra) rs#RA with
           | None => None
           | Some m3 => Some [Alloc stk 0 sz;
-                             Write stk (Int.unsigned ofs_link) (encode_val Mint32 (rs ESP));
-                             Write stk (Int.unsigned ofs_ra) (encode_val Mint32 (rs RA))]
+                             Write stk (Ptrofs.unsigned ofs_link) (encode_val Mptr (rs RSP));
+                             Write stk (Ptrofs.unsigned ofs_ra) (encode_val Mptr (rs RA))]
           end
       end
   | Pfreeframe sz ofs_ra ofs_link =>
-      match Mem.loadv Mint32 m (Val.add rs#ESP (Vint ofs_ra)) with
+      match Mem.loadv Mptr m (Val.offset_ptr rs#RSP ofs_ra) with
       | None => None
       | Some ra =>
-          match Mem.loadv Mint32 m (Val.add rs#ESP (Vint ofs_link)) with
+          match Mem.loadv Mptr m (Val.offset_ptr rs#RSP ofs_link) with
           | None => None
           | Some sp =>
-              match rs#ESP with
+              match rs#RSP with
               | Vptr stk ofs =>
                   match Mem.free m stk 0 sz with
                   | None => None
-                  | Some m' => match (Val.add rs#ESP (Vint ofs_ra)), (Val.add rs#ESP (Vint ofs_link)) with
+                  | Some m' => match (Val.offset_ptr rs#RSP ofs_ra), (Val.offset_ptr rs#RSP ofs_link) with
                                 Vptr b1 ofs1, Vptr b2 ofs2 =>
-                                  match Mem.loadbytes m b1 (Int.unsigned ofs1) (size_chunk Mint32), Mem.loadbytes m b2 (Int.unsigned ofs2) (size_chunk Mint32)
+                                  match Mem.loadbytes m b1 (Ptrofs.unsigned ofs1) (size_chunk Mptr), Mem.loadbytes m b2 (Ptrofs.unsigned ofs2) (size_chunk Mptr)
                                   with Some bytes1, Some bytes2=>
-                                     Some [Read b1 (Int.unsigned ofs1) (size_chunk Mint32) bytes1;
-                                           Read b2 (Int.unsigned ofs2) (size_chunk Mint32) bytes2;
+                                     Some [Read b1 (Ptrofs.unsigned ofs1) (size_chunk Mptr) bytes1;
+                                           Read b2 (Ptrofs.unsigned ofs2) (size_chunk Mptr) bytes2;
                                            Free [(stk, 0, sz)]]
                                    | _, _ => None
                                   end
@@ -205,9 +216,9 @@ Definition drf_instr (ge:genv) (c: code) (i: instruction) (rs: regset) (m: mem)
   | _ => Some [Free nil]
   end.
 
-Lemma store_stack_ev_elim m sp ty ofs v m' (SS: store_stack m sp ty ofs v = Some m'):
+(*Lemma store_stack_ev_elim m sp ty ofs v m' (SS: store_stack m sp ty ofs v = Some m'):
   exists b z, sp =Vptr b z /\
-  ev_elim m [Write b (Int.unsigned (Int.add z ofs)) (encode_val (chunk_of_type ty) v)] m'.
+  ev_elim m [Write b (Ptrofs.unsigned (Int.add z ofs)) (encode_val (chunk_of_type ty) v)] m'.
 Proof.
   destruct sp; try discriminate. unfold store_stack in SS.
   exists b, i; split; trivial.
@@ -224,9 +235,9 @@ Fixpoint store_args_ev_rec sp ofs args tys : option (list mem_event) :=
            match store_args_ev_rec sp (ofs+2) args' tys' with
              None => None
            | Some tailEvents =>
-               Some ((Write sp (Int.unsigned (Int.repr(Stacklayout.fe_ofs_arg + 4*(ofs+1))))
+               Some ((Write sp (Ptrofs.unsigned (Int.repr(Stacklayout.fe_ofs_arg + 4*(ofs+1))))
                               (encode_val (chunk_of_type Tint) (Vint (Int64.hiword n)))) ::
-                     (Write sp (Int.unsigned (Int.repr(Stacklayout.fe_ofs_arg + 4*ofs)))
+                     (Write sp (Ptrofs.unsigned (Int.repr(Stacklayout.fe_ofs_arg + 4*ofs)))
                             (encode_val (chunk_of_type Tint) (Vint (Int64.loword n)))) ::
                      tailEvents)
            end
@@ -235,7 +246,7 @@ Fixpoint store_args_ev_rec sp ofs args tys : option (list mem_event) :=
            match store_args_ev_rec sp (ofs+typesize ty') args' tys' with
              None => None
            | Some tailEvents =>
-               Some ((Write sp (Int.unsigned (Int.repr (Stacklayout.fe_ofs_arg + 4*ofs))) (encode_val (chunk_of_type ty') a'))
+               Some ((Write sp (Ptrofs.unsigned (Int.repr (Stacklayout.fe_ofs_arg + 4*ofs))) (encode_val (chunk_of_type ty') a'))
                       :: tailEvents)
            end
       end
@@ -347,7 +358,7 @@ induction args; intros tys; destruct tys; simpl; intros; try discriminate.
     econstructor. split. apply SB1. assumption.
 Qed.
 
-Definition store_args_events sp args tys := store_args_ev_rec sp 0 args tys.
+Definition store_args_events sp args tys := store_args_ev_rec sp 0 args tys.*)
 
 Lemma AR n: match n with
                   | 0 => 0
@@ -363,21 +374,21 @@ Inductive extcall_arg_ev (rs: regset) (m: mem): loc -> val -> list mem_event -> 
       extcall_arg_ev rs m (R r) (rs (preg_of r)) nil
   | extcall_arg_stack: forall ofs v ty bofs bytes chunk b z,
       bofs = Stacklayout.fe_ofs_arg + 4 * ofs ->
-      Val.add (rs (IR ESP)) (Vint (Int.repr bofs)) = Vptr b z ->
+      Val.offset_ptr (rs (IR RSP)) (Ptrofs.repr bofs) = Vptr b z ->
       chunk = chunk_of_type ty ->
 (*      Mem.loadv chunk m (Vptr b z) = Some v ->
-      extcall_arg_ev rs m (S Outgoing ofs ty) v [Read b (Int.unsigned z) (size_chunk chunk) (encode_val chunk v)].*)
-      (*(align_chunk (chunk_of_type ty) (Int.unsigned z)) ->*)
-      (align_chunk (chunk_of_type ty) | Int.unsigned z) -> (*(Int.add i (Int.repr (4 * ofs))))*)
-      Mem.loadbytes m b (Int.unsigned z) (size_chunk chunk) = Some bytes ->
+      extcall_arg_ev rs m (S Outgoing ofs ty) v [Read b (Ptrofs.unsigned z) (size_chunk chunk) (encode_val chunk v)].*)
+      (*(align_chunk (chunk_of_type ty) (Ptrofs.unsigned z)) ->*)
+      (align_chunk (chunk_of_type ty) | Ptrofs.unsigned z) -> (*(Int.add i (Int.repr (4 * ofs))))*)
+      Mem.loadbytes m b (Ptrofs.unsigned z) (size_chunk chunk) = Some bytes ->
       v= decode_val chunk bytes ->
-      extcall_arg_ev rs m (S Outgoing ofs ty) v [Read b (Int.unsigned z) (size_chunk chunk) bytes].
+      extcall_arg_ev rs m (S Outgoing ofs ty) v [Read b (Ptrofs.unsigned z) (size_chunk chunk) bytes].
 
 Lemma extcall_arg_extcall_arg_ev rs m l u (EA:extcall_arg rs m l u) : exists T, extcall_arg_ev rs m l u T.
 Proof.
   inv EA.
 + exists nil; constructor.
-+ remember (rs ESP) as p; destruct p; inv H0.
++ remember (rs RSP) as p; destruct p; inv H0.
   destruct (Mem.load_loadbytes _ _ _ _ _ H1) as [bytes [Bytes U]]. rewrite AR in *.
   destruct (Mem.load_valid_access _ _ _ _ _ H1) as [ ALGN].
   eexists; econstructor; try eassumption; try rewrite <- Heqp; reflexivity.
@@ -387,7 +398,7 @@ Lemma extcall_arg_ev_extcall_arg rs m l u T (EA:extcall_arg_ev rs m l u T): extc
 Proof.
   inv EA.
 + constructor.
-+ remember (rs ESP) as p; destruct p; inv H0. rewrite AR in *.
++ remember (rs RSP) as p; destruct p; inv H0. rewrite AR in *.
   econstructor. reflexivity. rewrite <- Heqp. simpl. rewrite AR.
   erewrite Mem.loadbytes_load; try reflexivity; eassumption.
 Qed.
@@ -551,26 +562,29 @@ Inductive eval_builtin_arg_ev: builtin_arg A -> val -> list mem_event -> Prop :=
   | eval_BA_ev_single: forall n,
       eval_builtin_arg_ev (BA_single n) (Vsingle n) nil
   | eval_BA_ev_loadstack: forall chunk ofs v b z bytes,
-      Mem.loadv chunk m (Val.add sp (Vint ofs)) = Some v ->
-      (align_chunk chunk | (Int.unsigned z)) ->
-      Mem.loadbytes m b (Int.unsigned z) (size_chunk chunk) = Some bytes ->
+      Mem.loadv chunk m (Val.offset_ptr sp ofs) = Some v ->
+      (align_chunk chunk | (Ptrofs.unsigned z)) ->
+      Mem.loadbytes m b (Ptrofs.unsigned z) (size_chunk chunk) = Some bytes ->
       v= decode_val chunk bytes ->
-      Val.add sp (Vint ofs) = Vptr b z ->
-      eval_builtin_arg_ev (BA_loadstack chunk ofs) v [Read b (Int.unsigned z) (size_chunk chunk) bytes]
+      Val.offset_ptr sp ofs = Vptr b z ->
+      eval_builtin_arg_ev (BA_loadstack chunk ofs) v [Read b (Ptrofs.unsigned z) (size_chunk chunk) bytes]
   | eval_BA_ev_addrstack: forall ofs,
-      eval_builtin_arg_ev (BA_addrstack ofs) (Val.add sp (Vint ofs)) nil
+      eval_builtin_arg_ev (BA_addrstack ofs) (Val.offset_ptr sp ofs) nil
   | eval_BA_ev_loadglobal: forall chunk id ofs v b z bytes,
       Mem.loadv chunk m (Senv.symbol_address ge id ofs) = Some v ->
-      (align_chunk chunk | (Int.unsigned z)) ->
-      Mem.loadbytes m b (Int.unsigned z) (size_chunk chunk) = Some bytes ->
+      (align_chunk chunk | (Ptrofs.unsigned z)) ->
+      Mem.loadbytes m b (Ptrofs.unsigned z) (size_chunk chunk) = Some bytes ->
       v= decode_val chunk bytes ->
       Senv.symbol_address ge id ofs = Vptr b z ->
-      eval_builtin_arg_ev (BA_loadglobal chunk id ofs) v [Read b (Int.unsigned z) (size_chunk chunk) bytes]
+      eval_builtin_arg_ev (BA_loadglobal chunk id ofs) v [Read b (Ptrofs.unsigned z) (size_chunk chunk) bytes]
   | eval_BA_ev_addrglobal: forall id ofs,
       eval_builtin_arg_ev (BA_addrglobal id ofs) (Senv.symbol_address ge id ofs) nil
   | eval_BA_ev_splitlong: forall hi lo vhi vlo Thi Tlo,
       eval_builtin_arg_ev hi vhi Thi -> eval_builtin_arg_ev lo vlo Tlo->
-      eval_builtin_arg_ev (BA_splitlong hi lo) (Val.longofwords vhi vlo) (Thi++Tlo).
+      eval_builtin_arg_ev (BA_splitlong hi lo) (Val.longofwords vhi vlo) (Thi++Tlo)
+  | eval_BA_ev_addptr: forall a1 a2 v1 v2 T1 T2,
+      eval_builtin_arg_ev a1 v1 T1 -> eval_builtin_arg_ev a2 v2 T2->
+      eval_builtin_arg_ev (BA_addptr a1 a2) (if Archi.ptr64 then Val.addl v1 v2 else Val.add v1 v2) (T1++T2).
 
 Lemma eval_builtin_arg_ev_determ: forall a v1 T1 (HT1:eval_builtin_arg_ev a v1 T1)
       v2 T2 (HT2:eval_builtin_arg_ev a v2 T2), v1=v2 /\ T1=T2.
@@ -578,6 +592,8 @@ Proof.
 induction a; intros; inv HT1; inv HT2; try solve [split; trivial].
 + rewrite H11 in H7; inv H7. rewrite H6 in H3; inv H3. split; trivial.
 + rewrite H12 in H8; inv H8. rewrite H7 in H4; inv H4. split; trivial.
++ destruct (IHa1 _ _ H2 _ _ H1); subst.
+  destruct (IHa2 _ _ H6 _ _ H4); subst. split; trivial.
 + destruct (IHa1 _ _ H2 _ _ H1); subst.
   destruct (IHa2 _ _ H6 _ _ H4); subst. split; trivial.
 Qed.
@@ -596,6 +612,8 @@ Proof.
   destruct (Mem.load_valid_access _ _ _ _ _ H) as [_ ALGN].
   eexists. econstructor; try eassumption; trivial. rewrite SA; trivial.
 + destruct IHeval_builtin_arg1 as [Thi HThi]. destruct IHeval_builtin_arg2 as [Tlo HTlo].
+  eexists. econstructor; eassumption.
++ destruct IHeval_builtin_arg1 as [T1 HT1]. destruct IHeval_builtin_arg2 as [T2 HT2].
   eexists. econstructor; eassumption.
 Qed.
 
@@ -676,6 +694,13 @@ Proof.
   destruct (EStrong2 _ _ E2) as [ML ELo]; subst mm'.
   split; trivial.
   constructor; eassumption.
++ destruct IHEV1 as [EL1 EStrong1]. destruct IHEV2 as [EL2 EStrong2].
+  split. eapply ev_elim_app; eassumption.
+  intros. apply ev_elim_split in H; destruct H as [m' [E1 E2]].
+  destruct (EStrong1 _ _ E1) as [MT EHi]; subst mm.
+  destruct (EStrong2 _ _ E2) as [ML ELo]; subst mm'.
+  split; trivial.
+  constructor; eassumption.
 Qed.
 
 Lemma eval_builtin_args_ev_elim_strong {A} ge (rs: A -> val) sp m al vl T (EV: eval_builtin_args_ev A ge rs sp m al vl T):
@@ -697,144 +722,146 @@ Qed.
 
 Inductive builtin_event: external_function -> mem -> list val -> list mem_event -> Prop :=
   BE_malloc: forall m n m'' b m'
-         (ALLOC: Mem.alloc m (-4) (Int.unsigned n) = (m'', b))
-         (ALGN : (align_chunk Mint32 | (-4)))
-         (ST: Mem.storebytes m'' b (-4) (encode_val Mint32 (Vint n)) = Some m'),
-         builtin_event EF_malloc m [Vint n]
-               [Alloc b (-4) (Int.unsigned n); Write b (-4) (encode_val Mint32 (Vint n))]
+         (ALLOC: Mem.alloc m (-size_chunk Mptr) (Ptrofs.unsigned n) = (m'', b))
+         (ALGN : (align_chunk Mptr | (-size_chunk Mptr)))
+         (ST: Mem.storebytes m'' b (-size_chunk Mptr) (encode_val Mptr (Vptrofs n)) = Some m'),
+         builtin_event EF_malloc m [Vptrofs n]
+               [Alloc b (-size_chunk Mptr) (Ptrofs.unsigned n);
+                Write b (-size_chunk Mptr) (encode_val Mptr (Vptrofs n))]
 | BE_free: forall m b lo bytes sz m'
-        (POS: Int.unsigned sz > 0)
-        (LB : Mem.loadbytes m b (Int.unsigned lo - 4) (size_chunk Mint32) = Some bytes)
-        (FR: Mem.free m b (Int.unsigned lo - 4) (Int.unsigned lo + Int.unsigned sz) = Some m')
-        (ALGN : (align_chunk Mint32 | Int.unsigned lo - 4))
-        (SZ : Vint sz = decode_val Mint32 bytes),
+        (POS: Ptrofs.unsigned sz > 0)
+        (LB : Mem.loadbytes m b (Ptrofs.unsigned lo - size_chunk Mptr) (size_chunk Mptr) = Some bytes)
+        (FR: Mem.free m b (Ptrofs.unsigned lo - size_chunk Mptr) (Ptrofs.unsigned lo + Ptrofs.unsigned sz) = Some m')
+        (ALGN : (align_chunk Mptr | Ptrofs.unsigned lo - size_chunk Mptr))
+        (SZ : Vptrofs sz = decode_val Mptr bytes),
         builtin_event EF_free m [Vptr b lo]
-              [Read b (Int.unsigned lo - 4) (size_chunk Mint32) bytes;
-               Free [(b,Int.unsigned lo - 4, Int.unsigned lo + Int.unsigned sz)]]
+              [Read b (Ptrofs.unsigned lo - size_chunk Mptr) (size_chunk Mptr) bytes;
+               Free [(b,Ptrofs.unsigned lo - size_chunk Mptr, Ptrofs.unsigned lo + Ptrofs.unsigned sz)]]
 | BE_memcpy: forall m al bsrc bdst sz bytes osrc odst m'
         (AL: al = 1 \/ al = 2 \/ al = 4 \/ al = 8)
         (POS : sz >= 0)
         (DIV : (al | sz))
-        (OSRC : sz > 0 -> (al | Int.unsigned osrc))
-        (ODST: sz > 0 -> (al | Int.unsigned odst))
+        (OSRC : sz > 0 -> (al | Ptrofs.unsigned osrc))
+        (ODST: sz > 0 -> (al | Ptrofs.unsigned odst))
         (RNG: bsrc <> bdst \/
-                Int.unsigned osrc = Int.unsigned odst \/
-                Int.unsigned osrc + sz <= Int.unsigned odst \/ Int.unsigned odst + sz <= Int.unsigned osrc)
-        (LB: Mem.loadbytes m bsrc (Int.unsigned osrc) sz = Some bytes)
-        (ST: Mem.storebytes m bdst (Int.unsigned odst) bytes = Some m'),
+                Ptrofs.unsigned osrc = Ptrofs.unsigned odst \/
+                Ptrofs.unsigned osrc + sz <= Ptrofs.unsigned odst \/ Ptrofs.unsigned odst + sz <= Ptrofs.unsigned osrc)
+        (LB: Mem.loadbytes m bsrc (Ptrofs.unsigned osrc) sz = Some bytes)
+        (ST: Mem.storebytes m bdst (Ptrofs.unsigned odst) bytes = Some m'),
         builtin_event (EF_memcpy sz al) m [Vptr bdst odst; Vptr bsrc osrc]
-              [Read bsrc (Int.unsigned osrc) sz bytes;
-               Write bdst (Int.unsigned odst) bytes]
+              [Read bsrc (Ptrofs.unsigned osrc) sz bytes;
+               Write bdst (Ptrofs.unsigned odst) bytes]
 | BE_EFexternal: forall name sg m vargs,
         I64Helpers.is_I64_helperS name sg ->
          builtin_event (EF_external name sg) m vargs []
 | BE_EFbuiltin: forall name sg m vargs, is_I64_builtinS name sg ->
          builtin_event (EF_builtin name sg) m vargs [].
 
-Lemma builtin_event_determ ef m vargs T1 (BE1: builtin_event ef m vargs T1) T2 (BE2: builtin_event ef m vargs T2): T1=T2.
-inv BE1; inv BE2; simpl in *; trivial.
-+ rewrite ALLOC0 in ALLOC; inv ALLOC; trivial.
-+ rewrite LB0 in LB; inv LB. rewrite <- SZ in SZ0; inv SZ0. trivial.
-+ rewrite LB0 in LB; inv LB; trivial.
+Lemma Vptrofs_inj : forall o1 o2, Vptrofs o1 = Vptrofs o2 ->
+  Ptrofs.unsigned o1 = Ptrofs.unsigned o2.
+Proof.
+  unfold Vptrofs; intros.
+  pose proof (Ptrofs.unsigned_range o1); pose proof (Ptrofs.unsigned_range o2).
+  destruct Archi.ptr64 eqn: H64.
+  - assert (Int64.unsigned (Ptrofs.to_int64 o1) = Int64.unsigned (Ptrofs.to_int64 o2)) by congruence.
+    unfold Ptrofs.to_int64 in *.
+    rewrite Ptrofs.modulus_eq64 in * by auto.
+    rewrite !Int64.unsigned_repr in * by (unfold Int64.max_unsigned; omega); auto.
+  - assert (Int.unsigned (Ptrofs.to_int o1) = Int.unsigned (Ptrofs.to_int o2)) by congruence.
+    unfold Ptrofs.to_int in *.
+    rewrite Ptrofs.modulus_eq32 in * by auto.
+    rewrite !Int.unsigned_repr in * by (unfold Int.max_unsigned; omega); auto.
 Qed.
 
+Lemma builtin_event_determ ef m vargs T1 (BE1: builtin_event ef m vargs T1) T2 (BE2: builtin_event ef m vargs T2): T1=T2.
+inversion BE1; inv BE2; try discriminate; simpl in *; trivial.
++ assert (Vptrofs n0 = Vptrofs n) as H by congruence.
+  rewrite H; rewrite (Vptrofs_inj _ _ H) in *.
+  rewrite ALLOC0 in ALLOC; inv ALLOC; trivial.
++ inv H5.
+  rewrite LB0 in LB; inv LB. rewrite <- SZ in SZ0. rewrite (Vptrofs_inj _ _ SZ0); trivial.
++ inv H3; inv H5.
+  rewrite LB0 in LB; inv LB; trivial.
+Qed.
+
+(* Is this too much copying? *)
 Inductive asm_ev_step ge : state -> mem -> list mem_event -> state -> mem -> Prop :=
   | asm_ev_step_internal:
-      forall b ofs f i rs m rs' m' lf T,
+      forall b ofs f i rs m1 m rs' m1' m' T,
       rs PC = Vptr b ofs ->
       Genv.find_funct_ptr ge b = Some (Internal f) ->
-      find_instr (Int.unsigned ofs) (fn_code f) = Some i ->
+      find_instr (Ptrofs.unsigned ofs) f.(fn_code) = Some i ->
       exec_instr ge f i rs m = Next rs' m' ->
       drf_instr ge (fn_code f) i rs m = Some T ->
-      asm_ev_step ge (State rs lf) m T (State rs' lf) m'
+      asm_ev_step ge (State rs m1) m T (State rs' m1') m'
   | asm_ev_step_builtin:
-      False -> (*We don't support builtins/helpers/vload/vstore etc yet*)
-      forall b ofs f ef args res rs m vargs t vres rs' m' lf T1 T2
-        (*(HFD: helper_functions_declared ge hf)*)
-         (NASS: ~ isInlinedAssembly ef)  (*NEW; we don't support inlined assembly yet*),
+      forall b ofs f ef args res rs m1 m vargs t vres rs' m1' m' T1 T2,
       rs PC = Vptr b ofs ->
       Genv.find_funct_ptr ge b = Some (Internal f) ->
-      find_instr (Int.unsigned ofs) f.(fn_code) = Some (Pbuiltin ef args res) ->
-      eval_builtin_args ge rs (rs ESP) m args vargs ->
+      find_instr (Ptrofs.unsigned ofs) f.(fn_code) = Some (Pbuiltin ef args res) ->
+      eval_builtin_args ge rs (rs RSP) m args vargs ->
       external_call ef ge vargs m t vres m' ->
-      ~ observableEF (*hf*) ef ->
       rs' = nextinstr_nf
              (set_res res vres
                (undef_regs (map preg_of (destroyed_by_builtin ef)) rs)) ->
-      eval_builtin_args_ev _ ge rs (rs ESP) m args vargs T1 ->
+      eval_builtin_args_ev _ ge rs (rs RSP) m args vargs T1 ->
       builtin_event ef m vargs T2 ->
-      asm_ev_step ge (State rs lf) m (T1++T2) (State rs' lf) m'
-  | asm_ev_step_to_external:
-      forall b ef args rs m lf T
-      (*(HFD: helper_functions_declared ge hf)*),
-      rs PC = Vptr b Int.zero ->
-      Genv.find_funct_ptr ge b = Some (External ef) ->
-      extcall_arguments rs m (ef_sig ef) args ->
-      extcall_arguments_ev rs m (ef_sig ef) args T ->
-      asm_ev_step ge (State rs lf) m T (Asm_CallstateOut ef args rs lf) m
+      asm_ev_step ge (State rs m1) m (T1++T2) (State rs' m1') m'.
 
-  | asm_ev_step_external: (*really, a helper-step*)
-      False -> (*We don't support builtins/helpers/vload/vstore etc yet*)
-      forall b callee args res rs m t rs' m' lf T
-      (*(HFD: helper_functions_declared ge hf)*)
-      (OBS: EFisHelper (*hf*) callee),
-      rs PC = Vptr b Int.zero ->
-      Genv.find_funct_ptr ge b = Some (External callee) ->
-      extcall_arguments rs m (ef_sig callee) args ->
-      external_call callee ge args m t res m' ->
-      rs' = (set_pair (loc_external_result (ef_sig callee)) res rs) #PC <- (rs RA) ->
-      builtin_event  callee m args T ->
-      asm_ev_step ge (Asm_CallstateOut callee args rs lf) m T (State rs' lf) m'
-  (*NOTE [loader]*)
-  | asm_ev_initialize_call:
-      forall m args tys retty m1 stk m2 fb z T
-      (*(HFD: helper_functions_declared ge hf)*),
-      args_len_rec args tys = Some z ->
-      Mem.alloc m 0 (4*z) = (m1, stk) ->
-      store_args m1 stk args tys = Some m2 ->
-      store_args_events stk args tys = Some T ->
-      let rs0 := (Pregmap.init Vundef)
-                  #PC <- (Vptr fb Int.zero)
-                  #RA <- Vzero
-                  # ESP <- (Vptr stk Int.zero) in
-      asm_ev_step ge (Asm_CallstateIn fb args tys retty) m (Alloc stk 0 (4*z) :: T)
-               (State rs0 (mk_load_frame stk retty)) m2.
-
-Lemma asm_ev_ax1 g (*(HFD: helper_functions_declared g hf)*):
-  forall c m T c' m' (EStep:asm_ev_step g c m T c' m'), corestep (Asm_mem_sem (*hf*)) g c m c' m'.
+Lemma asm_ev_ax1 prog (*(HFD: helper_functions_declared g hf)*):
+  forall c m T c' m' (EStep:asm_ev_step (Genv.globalenv prog) c m T c' m'), corestep (Asm_mem_sem prog (*hf*)) (Genv.globalenv prog) c m c' m'.
 Proof.
  induction 1; try contradiction.
 + destruct i; inv H2;
-  try solve[eapply asm_exec_step_internal; try eassumption; reflexivity].
-(*+ (*builtin*) eapply asm_exec_step_builtin; eassumption.*)
-+ (*step-to_callstateOut*) eapply asm_exec_step_to_external; eassumption.
-(*+ (*step_from-callstateOut*) eapply asm_exec_step_external; try eassumption.*)
-+ (*loadframe*) eapply asm_exec_initialize_call; try eassumption.
+  solve[eapply coreify; [eapply exec_step_internal; try eassumption; reflexivity |
+    simpl; unfold fundef; rewrite H, H0; destruct (Ptrofs.eq_dec _ _); reflexivity]].
++ (* builtin *) eapply coreify; [eapply exec_step_builtin; try eassumption; reflexivity |
+    simpl; unfold fundef; rewrite H, H0; destruct (Ptrofs.eq_dec _ _); reflexivity].
 Qed.
 
-Lemma asm_ev_ax2 g: forall c m c' m' (CS:corestep (Asm_mem_sem (*hf*)) g c m c' m'),
-   exists T, asm_ev_step g c m T c' m'.
-Proof. induction 1; try contradiction.
-+ destruct i; inv H2;
+Lemma asm_ev_ax2 prog: forall c m c' m' (CS:corestep (Asm_mem_sem prog (*hf*)) (Genv.globalenv prog) c m c' m'),
+   exists T, asm_ev_step (Genv.globalenv prog) c m T c' m'.
+Proof. inversion 1; subst.
+destruct c as [rs ?], c' as [rs' ?]; simpl in H.
+inv H.
++ set (g := Genv.globalenv prog) in *.
+  destruct i; inv H9;
   try solve [eexists; eapply asm_ev_step_internal; try eassumption; reflexivity].
-  - unfold exec_load in H4.
-    remember (Mem.loadv Mint32 m (eval_addrmode g a rs)) as p.
+  - unfold exec_load in H1.
+    remember (Mem.loadv Mint32 m (eval_addrmode _ a rs)) as p.
     destruct p; try discriminate; symmetry in Heqp.
-    remember (eval_addrmode g a rs) as q.
+    remember (eval_addrmode _ a rs) as q.
     destruct q; try discriminate.
     destruct (Mem.load_loadbytes _ _ _ _ _ Heqp) as [bytes [LB V]]; simpl in LB.
     eexists; eapply asm_ev_step_internal; try eassumption; simpl.
     * unfold exec_load. rewrite <- Heqq, Heqp. trivial.
     * rewrite <- Heqq, LB. reflexivity.
-  - unfold exec_store in H4.
-    remember (Mem.storev Mint32 m (eval_addrmode g a rs) (rs rs0)) as p.
+  - unfold exec_load in H1.
+    remember (Mem.loadv Mint64 m (eval_addrmode _ a rs)) as p.
     destruct p; try discriminate; symmetry in Heqp.
-    remember (eval_addrmode g a rs) as q.
+    remember (eval_addrmode _ a rs) as q.
+    destruct q; try discriminate.
+    destruct (Mem.load_loadbytes _ _ _ _ _ Heqp) as [bytes [LB V]]; simpl in LB.
+    eexists; eapply asm_ev_step_internal; try eassumption; simpl.
+    * unfold exec_load. rewrite <- Heqq, Heqp. trivial.
+    * rewrite <- Heqq, LB. reflexivity.
+  - unfold exec_store in H1.
+    remember (Mem.storev Mint32 m (eval_addrmode _ a rs) (rs rs0)) as p.
+    destruct p; try discriminate; symmetry in Heqp.
+    remember (eval_addrmode _ a rs) as q.
     destruct q; try discriminate.
     eexists; eapply asm_ev_step_internal; try eassumption; simpl.
     * unfold exec_store. rewrite <- Heqq, Heqp. trivial.
     * rewrite <- Heqq. reflexivity.
-  - unfold exec_load in H4.
+  - unfold exec_store in H1.
+    remember (Mem.storev Mint64 m (eval_addrmode _ a rs) (rs rs0)) as p.
+    destruct p; try discriminate; symmetry in Heqp.
+    remember (eval_addrmode _ a rs) as q.
+    destruct q; try discriminate.
+    eexists; eapply asm_ev_step_internal; try eassumption; simpl.
+    * unfold exec_store. rewrite <- Heqq, Heqp. trivial.
+    * rewrite <- Heqq. reflexivity.
+  - unfold exec_load in H1.
     remember (Mem.loadv Mfloat64 m (eval_addrmode g a rs)) as p.
     destruct p; try discriminate; symmetry in Heqp.
     remember (eval_addrmode g a rs) as q.
@@ -843,7 +870,7 @@ Proof. induction 1; try contradiction.
     eexists; eapply asm_ev_step_internal; try eassumption; simpl.
     * unfold exec_load. rewrite <- Heqq, Heqp. trivial.
     * rewrite <- Heqq, LB. reflexivity.
-  - unfold exec_store in H4.
+  - unfold exec_store in H1.
     remember (Mem.storev Mfloat64 m (eval_addrmode g a rs) (rs r1)) as p.
     destruct p; try discriminate; symmetry in Heqp.
     remember (eval_addrmode g a rs) as q.
@@ -851,7 +878,7 @@ Proof. induction 1; try contradiction.
     eexists; eapply asm_ev_step_internal; try eassumption; simpl.
     * unfold exec_store. rewrite <- Heqq, Heqp. trivial.
     * rewrite <- Heqq. reflexivity.
-  - unfold exec_load in H4.
+  - unfold exec_load in H1.
     remember (Mem.loadv Mfloat32 m (eval_addrmode g a rs)) as p.
     destruct p; try discriminate; symmetry in Heqp.
     remember (eval_addrmode g a rs) as q.
@@ -860,7 +887,7 @@ Proof. induction 1; try contradiction.
     eexists; eapply asm_ev_step_internal; try eassumption; simpl.
     * unfold exec_load. rewrite <- Heqq, Heqp. trivial.
     * rewrite <- Heqq, LB. reflexivity.
-  - unfold exec_store in H4.
+  - unfold exec_store in H1.
     remember (Mem.storev Mfloat32 m (eval_addrmode g a rs) (rs r1)) as p.
     destruct p; try discriminate; symmetry in Heqp.
     remember (eval_addrmode g a rs) as q.
@@ -868,7 +895,7 @@ Proof. induction 1; try contradiction.
     eexists; eapply asm_ev_step_internal; try eassumption; simpl.
     * unfold exec_store. rewrite <- Heqq, Heqp. trivial.
     * rewrite <- Heqq. reflexivity.
-  - unfold exec_load in H4.
+  - unfold exec_load in H1.
     remember (Mem.loadv Mfloat64 m (eval_addrmode g a rs)) as p.
     destruct p; try discriminate; symmetry in Heqp.
     remember (eval_addrmode g a rs) as q.
@@ -877,7 +904,7 @@ Proof. induction 1; try contradiction.
     eexists; eapply asm_ev_step_internal; try eassumption; simpl.
     * unfold exec_load. rewrite <- Heqq, Heqp. trivial.
     * rewrite <- Heqq, LB. reflexivity.
-  - unfold exec_store in H4.
+  - unfold exec_store in H1.
     remember (Mem.storev Mfloat64 m (eval_addrmode g a rs) (rs ST0)) as p.
     destruct p; try discriminate; symmetry in Heqp.
     remember (eval_addrmode g a rs) as q.
@@ -885,7 +912,7 @@ Proof. induction 1; try contradiction.
     eexists; eapply asm_ev_step_internal; try eassumption; simpl.
     * unfold exec_store. rewrite <- Heqq, Heqp. trivial.
     * rewrite <- Heqq. reflexivity.
-  - unfold exec_load in H4.
+  - unfold exec_load in H1.
     remember (Mem.loadv Mfloat32 m (eval_addrmode g a rs)) as p.
     destruct p; try discriminate; symmetry in Heqp.
     remember (eval_addrmode g a rs) as q.
@@ -894,7 +921,7 @@ Proof. induction 1; try contradiction.
     eexists; eapply asm_ev_step_internal; try eassumption; simpl.
     * unfold exec_load. rewrite <- Heqq, Heqp. trivial.
     * rewrite <- Heqq, LB. reflexivity.
-  - unfold exec_store in H4.
+  - unfold exec_store in H1.
     remember (Mem.storev Mfloat32 m (eval_addrmode g a rs) (rs ST0)) as p.
     destruct p; try discriminate; symmetry in Heqp.
     remember (eval_addrmode g a rs) as q.
@@ -902,7 +929,7 @@ Proof. induction 1; try contradiction.
     eexists; eapply asm_ev_step_internal; try eassumption; simpl.
     * unfold exec_store. rewrite <- Heqq, Heqp. trivial.
     * rewrite <- Heqq. reflexivity.
-  - unfold exec_store in H4.
+  - unfold exec_store in H1.
     remember (Mem.storev Mint8unsigned m (eval_addrmode g a rs) (rs rs0)) as p.
     destruct p; try discriminate; symmetry in Heqp.
     remember (eval_addrmode g a rs) as q.
@@ -910,7 +937,7 @@ Proof. induction 1; try contradiction.
     eexists; eapply asm_ev_step_internal; try eassumption; simpl.
     * unfold exec_store. rewrite <- Heqq, Heqp. trivial.
     * rewrite <- Heqq. reflexivity.
-  - unfold exec_store in H4.
+  - unfold exec_store in H1.
     remember (Mem.storev Mint16unsigned m (eval_addrmode g a rs) (rs rs0)) as p.
     destruct p; try discriminate; symmetry in Heqp.
     remember (eval_addrmode g a rs) as q.
@@ -918,7 +945,7 @@ Proof. induction 1; try contradiction.
     eexists; eapply asm_ev_step_internal; try eassumption; simpl.
     * unfold exec_store. rewrite <- Heqq, Heqp. trivial.
     * rewrite <- Heqq. reflexivity.
-  - unfold exec_load in H4.
+  - unfold exec_load in H1.
     remember (Mem.loadv Mint8unsigned m (eval_addrmode g a rs)) as p.
     destruct p; try discriminate; symmetry in Heqp.
     remember (eval_addrmode g a rs) as q.
@@ -927,7 +954,7 @@ Proof. induction 1; try contradiction.
     eexists; eapply asm_ev_step_internal; try eassumption; simpl.
     * unfold exec_load. rewrite <- Heqq, Heqp. trivial.
     * rewrite <- Heqq, LB. reflexivity.
-  - unfold exec_load in H4.
+  - unfold exec_load in H1.
     remember (Mem.loadv Mint8signed m (eval_addrmode g a rs)) as p.
     destruct p; try discriminate; symmetry in Heqp.
     remember (eval_addrmode g a rs) as q.
@@ -936,7 +963,7 @@ Proof. induction 1; try contradiction.
     eexists; eapply asm_ev_step_internal; try eassumption; simpl.
     * unfold exec_load. rewrite <- Heqq, Heqp. trivial.
     * rewrite <- Heqq, LB. reflexivity.
-  - unfold exec_load in H4.
+  - unfold exec_load in H1.
     remember (Mem.loadv Mint16unsigned m (eval_addrmode g a rs)) as p.
     destruct p; try discriminate; symmetry in Heqp.
     remember (eval_addrmode g a rs) as q.
@@ -945,7 +972,7 @@ Proof. induction 1; try contradiction.
     eexists; eapply asm_ev_step_internal; try eassumption; simpl.
     * unfold exec_load. rewrite <- Heqq, Heqp. trivial.
     * rewrite <- Heqq, LB. reflexivity.
-  - unfold exec_load in H4.
+  - unfold exec_load in H1.
     remember (Mem.loadv Mint16signed m (eval_addrmode g a rs)) as p.
     destruct p; try discriminate; symmetry in Heqp.
     remember (eval_addrmode g a rs) as q.
@@ -954,8 +981,8 @@ Proof. induction 1; try contradiction.
     eexists; eapply asm_ev_step_internal; try eassumption; simpl.
     * unfold exec_load. rewrite <- Heqq, Heqp. trivial.
     * rewrite <- Heqq, LB. reflexivity.
-  - unfold exec_load in H4.
-    remember (Mem.loadv Many32 m (eval_addrmode g a rs)) as p.
+  - unfold exec_load in H1.
+    remember (Mem.loadv _ m (eval_addrmode g a rs)) as p.
     destruct p; try discriminate; symmetry in Heqp.
     remember (eval_addrmode g a rs) as q.
     destruct q; try discriminate.
@@ -963,15 +990,15 @@ Proof. induction 1; try contradiction.
     eexists; eapply asm_ev_step_internal; try eassumption; simpl.
     * unfold exec_load. rewrite <- Heqq, Heqp. trivial.
     * rewrite <- Heqq, LB. reflexivity.
-  - unfold exec_store in H4.
-    remember (Mem.storev Many32 m (eval_addrmode g a rs) (rs rs0)) as p.
+  - unfold exec_store in H1.
+    remember (Mem.storev _ m (eval_addrmode g a rs) (rs rs0)) as p.
     destruct p; try discriminate; symmetry in Heqp.
     remember (eval_addrmode g a rs) as q.
     destruct q; try discriminate.
     eexists; eapply asm_ev_step_internal; try eassumption; simpl.
     * unfold exec_store. rewrite <- Heqq, Heqp. trivial.
     * rewrite <- Heqq. reflexivity.
-  - unfold exec_load in H4.
+  - unfold exec_load in H1.
     remember (Mem.loadv Many64 m (eval_addrmode g a rs)) as p.
     destruct p; try discriminate; symmetry in Heqp.
     remember (eval_addrmode g a rs) as q.
@@ -980,7 +1007,7 @@ Proof. induction 1; try contradiction.
     eexists; eapply asm_ev_step_internal; try eassumption; simpl.
     * unfold exec_load. rewrite <- Heqq, Heqp. trivial.
     * rewrite <- Heqq, LB. reflexivity.
-  - unfold exec_store in H4.
+  - unfold exec_store in H1.
     remember (Mem.storev Many64 m (eval_addrmode g a rs) (rs r1)) as p.
     destruct p; try discriminate; symmetry in Heqp.
     remember (eval_addrmode g a rs) as q.
@@ -989,19 +1016,19 @@ Proof. induction 1; try contradiction.
     * unfold exec_store. rewrite <- Heqq, Heqp. trivial.
     * rewrite <- Heqq. reflexivity.
   - (*Pallocframe*)
-    remember (Mem.alloc m 0 sz) as alloc; destruct alloc as [m1 stk].
-    remember (Mem.store Mint32 m1 stk (Int.unsigned (Int.add Int.zero ofs_link)) (rs ESP)) as p; destruct p; try discriminate.
-    remember (Mem.store Mint32 m0 stk (Int.unsigned (Int.add Int.zero ofs_ra)) (rs RA)) as q; destruct q; try discriminate.
-    inv H4.
+    remember (Mem.alloc m 0 sz) as alloc; destruct alloc as [ma stk].
+    remember (Mem.store Mptr ma stk (Ptrofs.unsigned (Ptrofs.add Ptrofs.zero ofs_link)) (rs RSP)) as p; destruct p; try discriminate.
+    remember (Mem.store Mptr m2 stk (Ptrofs.unsigned (Ptrofs.add Ptrofs.zero ofs_ra)) (rs RA)) as q; destruct q; try discriminate.
+    inv H1.
     eexists.
     eapply asm_ev_step_internal; try eassumption; simpl.
     * rewrite <- Heqalloc, <- Heqp, <- Heqq. reflexivity.
     * rewrite <- Heqalloc, <- Heqp, <- Heqq. reflexivity.
   - (*Pfreeframe*)
-    remember (Mem.loadv Mint32 m (Val.add (rs ESP) (Vint ofs_ra))) as p; destruct p; try discriminate.
-    remember (Mem.loadv Mint32 m (Val.add (rs ESP) (Vint ofs_link))) as q; destruct q; try discriminate.
-    remember (rs ESP) as w; destruct w; try discriminate.
-    remember (Mem.free m b0 0 sz) as r; destruct r; try discriminate. inv H4.
+    remember (Mem.loadv Mptr m (Val.offset_ptr (rs RSP) ofs_ra)) as p; destruct p; try discriminate.
+    remember (Mem.loadv Mptr m (Val.offset_ptr (rs RSP) ofs_link)) as q; destruct q; try discriminate.
+    remember (rs RSP) as w; destruct w; try discriminate.
+    remember (Mem.free m b0 0 sz) as r; destruct r; try discriminate. inv H1.
     symmetry in Heqp, Heqq. simpl in *.
     destruct (Mem.load_loadbytes _ _ _ _ _ Heqp) as [bytes1 [Bytes1 LD1]].
     destruct (Mem.load_loadbytes _ _ _ _ _ Heqq) as [bytes2 [Bytes2 LD2]].
@@ -1011,46 +1038,59 @@ Proof. induction 1; try contradiction.
       rewrite Heqp, Heqq, <- Heqr. trivial.
     * rewrite <- Heqw in *. simpl in *.
       rewrite Heqp, Heqq, <- Heqr, Bytes1, Bytes2. reflexivity.
-(*+ (*builtin*)
++ (*builtin*)
   exploit eval_builtin_args_eval_builtin_args_ev. eassumption. intros [T HT].
-  destruct ef; simpl in *; try solve [elim H4; trivial].
+  (* We need to know that we've caught all the memory-affecting builtins. *)
+  destruct ef; simpl in *.
   - exists (T ++ nil).
     eapply asm_ev_step_builtin; try eassumption. simpl; trivial.
-    eapply BE_EFexternal. destruct (I64Helpers.is_I64_helperS_dec name sg); trivial. elim H4; trivial.
+    eapply BE_EFexternal. destruct (I64Helpers.is_I64_helperS_dec name sg); trivial. admit.
+    (* Should we restrict builtin externals to helpers? Should those go under EF_builtin? *)
   - exists (T ++ nil).
     eapply asm_ev_step_builtin; try eassumption. simpl; trivial.
-    eapply BE_EFbuiltin. destruct (is_I64_builtinS_dec name sg); trivial. elim H4; trivial.
+    eapply BE_EFbuiltin. destruct (is_I64_builtinS_dec name sg); trivial. admit.
+  - admit. (* EFruntime *)
+  - admit. (* vload *)
+  - admit. (* vstore *)
   - (*malloc*)
-    inv H3. destruct (Mem.store_valid_access_3 _ _ _ _ _ _ H7) as [_ ALGN].
-    specialize (Mem.store_storebytes _ _ _ _ _ _ H7). intros.
+    inv H10. destruct (Mem.store_valid_access_3 _ _ _ _ _ _ H1) as [_ ALGN].
+    specialize (Mem.store_storebytes _ _ _ _ _ _ H1). intros.
     eexists. eapply asm_ev_step_builtin; try eassumption; simpl; trivial.
     * econstructor; try eassumption.
     * econstructor; eassumption.
   - (*free*)
-    inv H3. destruct (Mem.load_valid_access _ _ _ _ _ H6) as [_ ALGN].
-    destruct (Mem.load_loadbytes _ _ _ _ _ H6) as [bytes [LB V]].
+    inv H10. destruct (Mem.load_valid_access _ _ _ _ _ H) as [_ ALGN].
+    destruct (Mem.load_loadbytes _ _ _ _ _ H) as [bytes [LB V]].
     eexists. eapply asm_ev_step_builtin; try eassumption; simpl; trivial.
     * econstructor; try eassumption.
     * econstructor; eassumption.
   - (*memcpy*)
-    inv H3.
+    inv H10.
     eexists. eapply asm_ev_step_builtin; try eassumption; simpl; trivial.
     * econstructor; try eassumption.
-    * econstructor; eassumption.*)
-+ (*step-to_callstateOut*)
-   exploit extcall_arguments_extcall_arguments_ev. eassumption. intros [T HT].
-   exists T. econstructor; eassumption.
-(*+ (*step_from-callstateOut*)
-   exists nil.
-   econstructor; try eassumption. inv H1.
-   destruct callee; simpl in *; try solve [contradiction].
-   eapply BE_EFexternal. trivial.
-   eapply BE_EFbuiltin. trivial. *)
-+ (*loadframe*)
-  unfold store_args in H1.
-  destruct (store_args_ev_elim _ _ _ _ _ _ H1) as [T [HT EV]].
-  eexists. eapply asm_ev_initialize_call; eassumption.
-Qed.
+    * econstructor; eassumption.
+  - inv H10.
+    exists (T ++ nil).
+    eapply asm_ev_step_builtin; eauto.
+    constructor; eauto.
+    admit. (* EF_annot *)
+  - inv H10.
+    exists (T ++ nil).
+    eapply asm_ev_step_builtin; eauto.
+    constructor; eauto.
+    admit. (* EF_annot_val *)
+  - admit. (* inline assembly *)
+  - inv H10.
+    exists (T ++ nil).
+    eapply asm_ev_step_builtin; eauto.
+    constructor; eauto.
+    admit. (* EF_debug *)
++ simpl in H0.
+  rewrite H5, H6 in H0.
+  destruct (Ptrofs.eq_dec _ _); [|contradiction].
+  destruct ef; try discriminate.
+  (* Are there "external steps" that don't count as external for at_external? *)
+Admitted.
 
 Lemma asm_ev_fun g: forall c m T' c' m' T'' c'' m''
     (Estep': asm_ev_step g c m T' c' m') (Estep'': asm_ev_step g c m T'' c'' m''), T' = T''.
@@ -1059,16 +1099,15 @@ inv Estep'; inv Estep''; trivial; try contradiction.
 + rewrite H in H6; inv H6. rewrite H0 in H7; inv H7.
   rewrite H1 in H8; inv H8. rewrite H2 in H9; inv H9.
   rewrite H3 in H14; inv H14. trivial.
-(*+ rewrite H in H7; inv H7. rewrite H0 in H7; inv H7.
-  rewrite H1 in H8; inv H8. simpl in *; discriminate. *)
 + rewrite H in H6; inv H6. rewrite H0 in H7; inv H7.
-(*+ rewrite H in H9; inv H9. rewrite H0 in H10; inv H10.
-  rewrite H1 in H11; inv H11. simpl in *; discriminate. *)
-(*+ rewrite H9 in H; inv H. rewrite H10 in H0; inv H0.
-  rewrite H11 in H1; inv H1.
-  exploit eval_builtin_args_ev_determ. apply H16. apply H6. intros [Y X]; subst.
-  f_equal. eapply builtin_event_determ; eassumption.*)
-(*+ rewrite H9 in H; inv H. rewrite H0 in H10; discriminate.*)
+  rewrite H1 in H8; inv H8. simpl in *; discriminate.
++ rewrite H in H8; inv H8. rewrite H0 in H9; inv H9.
+  rewrite H1 in H10; inv H10. simpl in *; discriminate.
++ rewrite H in H8; inv H8. rewrite H0 in H9; inv H9.
+  rewrite H1 in H10; inv H10.
+  exploit eval_builtin_args_ev_determ. apply H14. apply H5. intros [Y X]; subst.
+  f_equal. eapply builtin_event_determ; eassumption.
+(*(*+ rewrite H9 in H; inv H. rewrite H0 in H10; discriminate.*)
 + rewrite H5 in H; inv H. rewrite H0 in H6; discriminate.
 (*+ rewrite H5 in H; inv H. rewrite H0 in H6; inv H6.*)
 + rewrite H5 in H; inv H. rewrite H6 in H0; inv H0.
@@ -1077,7 +1116,7 @@ inv Estep'; inv Estep''; trivial; try contradiction.
 (*+ rewrite H7 in H; inv H. eapply builtin_event_determ; eassumption. *)
 + (*loadframe*)
   rewrite H7 in H; inv H. rewrite H12 in H0; inv H0.
-  rewrite H13 in H1; inv H1. rewrite H14 in H2; inv H2. reflexivity.
+  rewrite H13 in H1; inv H1. rewrite H14 in H2; inv H2. reflexivity.*)
 Qed.
 
 Lemma asm_ev_elim g: forall c m T c' m' (Estep: asm_ev_step g c m T c' m'), ev_elim m T m'.
@@ -1093,8 +1132,23 @@ induction 1; intros; try contradiction.
     destruct (Mem.load_loadbytes _ _ _ _ _ Heqp) as [bytes [LB V]]; simpl in LB.
     rewrite LB in H4; inv H4. inv H5.
     constructor; simpl; trivial.
+  - unfold exec_load in H5.
+    remember (Mem.loadv Mint64 m (eval_addrmode g a rs)) as p.
+    destruct p; try discriminate; symmetry in Heqp.
+    remember (eval_addrmode g a rs) as q.
+    destruct q; try discriminate.
+    destruct (Mem.load_loadbytes _ _ _ _ _ Heqp) as [bytes [LB V]]; simpl in LB.
+    rewrite LB in H4; inv H4. inv H5.
+    constructor; simpl; trivial.
   - unfold exec_store in H5.
     remember (Mem.storev Mint32 m (eval_addrmode g a rs) (rs rs0)) as p.
+    destruct p; try discriminate; symmetry in Heqp.
+    remember (eval_addrmode g a rs) as q.
+    destruct q; try discriminate. inv H5; inv H4.
+    apply Mem.store_storebytes in Heqp.
+    econstructor. split; simpl; trivial. eassumption.
+  - unfold exec_store in H5.
+    remember (Mem.storev Mint64 m (eval_addrmode g a rs) (rs rs0)) as p.
     destruct p; try discriminate; symmetry in Heqp.
     remember (eval_addrmode g a rs) as q.
     destruct q; try discriminate. inv H5; inv H4.
@@ -1206,11 +1260,25 @@ induction 1; intros; try contradiction.
     destruct (Mem.load_loadbytes _ _ _ _ _ Heqp) as [bytes [LB V]]; simpl in LB.
     rewrite LB in H4; inv H4. inv H5.
     constructor; simpl; trivial.
-  - destruct (Val.divu (rs EAX) (rs # EDX <- Vundef r1)); inv H5.
-    destruct (Val.modu (rs EAX) (rs # EDX <- Vundef r1)); inv H3.
+  - destruct (rs RDX); inv H5.
+    destruct (rs RAX); inv H3.
+    destruct (rs r1); inv H4.
+    destruct (Int.divmodu2 _ _ _) as [[]|]; inv H3.
     eexists; simpl; split; reflexivity.
-  - destruct (Val.divs (rs EAX) (rs # EDX <- Vundef r1)); inv H5.
-    destruct (Val.mods (rs EAX) (rs # EDX <- Vundef r1)); inv H3.
+  - destruct (rs RDX); inv H5.
+    destruct (rs RAX); inv H3.
+    destruct (rs r1); inv H4.
+    destruct (Int64.divmodu2 _ _ _) as [[]|]; inv H3.
+    eexists; simpl; split; reflexivity.
+  - destruct (rs RDX); inv H5.
+    destruct (rs RAX); inv H3.
+    destruct (rs r1); inv H4.
+    destruct (Int.divmods2 _ _ _) as [[]|]; inv H3.
+    eexists; simpl; split; reflexivity.
+  - destruct (rs RDX); inv H5.
+    destruct (rs RAX); inv H3.
+    destruct (rs r1); inv H4.
+    destruct (Int64.divmods2 _ _ _) as [[]|]; inv H3.
     eexists; simpl; split; reflexivity.
   - destruct (eval_testcond c rs); inv H5.
     * destruct b0; inv H3; eexists; simpl; split; reflexivity.
@@ -1233,11 +1301,11 @@ induction 1; intros; try contradiction.
     * destruct (eval_testcond c2 rs); inv H4; try solve [eexists; simpl; split; reflexivity].
   - destruct (rs r); inv H5.
     destruct (list_nth_z tbl (Int.unsigned i)); inv H3.
-    unfold goto_label in H4. rewrite H in *.
+    unfold goto_label in H4. rewrite !Pregmap.gso, H in H4 by discriminate.
     destruct (label_pos l 0 (fn_code f)); inv H4.
     eexists; simpl; split; reflexivity.
   - unfold exec_load in H5.
-    remember (Mem.loadv Many32 m (eval_addrmode g a rs)) as p.
+    remember (Mem.loadv _ m (eval_addrmode g a rs)) as p.
     destruct p; try discriminate; symmetry in Heqp.
     remember (eval_addrmode g a rs) as q.
     destruct q; try discriminate.
@@ -1245,7 +1313,7 @@ induction 1; intros; try contradiction.
     rewrite LB in H4; inv H4. inv H5.
     constructor; simpl; trivial.
   - unfold exec_store in H5.
-    remember (Mem.storev Many32 m (eval_addrmode g a rs) (rs rs0)) as p.
+    remember (Mem.storev _ m (eval_addrmode g a rs) (rs rs0)) as p.
     destruct p; try discriminate; symmetry in Heqp.
     remember (eval_addrmode g a rs) as q.
     destruct q; try discriminate. inv H5; inv H4.
@@ -1267,27 +1335,27 @@ induction 1; intros; try contradiction.
     apply Mem.store_storebytes in Heqp.
     econstructor. split; simpl; trivial. eassumption.
   - (*Pallocframe*)
-    remember (Mem.alloc m 0 sz) as a; symmetry in Heqa; destruct a as [m1 stk].
-    remember (Mem.store Mint32 m1 stk
-         (Int.unsigned (Int.add Int.zero ofs_link))
-         (rs ESP)) as p.
+    remember (Mem.alloc m 0 sz) as a; symmetry in Heqa; destruct a as [ma stk].
+    remember (Mem.store Mptr ma stk
+         (Ptrofs.unsigned (Ptrofs.add Ptrofs.zero ofs_link))
+         (rs RSP)) as p.
     destruct p; try discriminate; symmetry in Heqp.
-    remember (Mem.store Mint32 m0 stk (Int.unsigned (Int.add Int.zero ofs_ra))
+    remember (Mem.store Mptr m0 stk (Ptrofs.unsigned (Ptrofs.add Ptrofs.zero ofs_ra))
          (rs RA)) as q.
     destruct q; try discriminate; symmetry in Heqq. inv H5; inv H4.
     apply Mem.store_storebytes in Heqp.
     apply Mem.store_storebytes in Heqq.
-    rewrite Int.add_zero_l in *.
+    rewrite Ptrofs.add_zero_l in *.
     econstructor. split. eassumption.
     econstructor. split. eassumption.
     econstructor. split. eassumption.
     econstructor.
   - (*Pfreeframe*)
-    remember (Mem.loadv Mint32 m (Val.add (rs ESP) (Vint ofs_ra))) as p.
+    remember (Mem.loadv Mptr m (Val.offset_ptr (rs RSP) ofs_ra)) as p.
     destruct p; try discriminate; symmetry in Heqp.
-    remember (Mem.loadv Mint32 m (Val.add (rs ESP) (Vint ofs_link))) as q.
+    remember (Mem.loadv Mptr m (Val.offset_ptr (rs RSP) ofs_link)) as q.
     destruct q; try discriminate; symmetry in Heqq.
-    remember (rs ESP) as w; destruct w; try discriminate.
+    remember (rs RSP) as w; destruct w; try discriminate.
     remember (Mem.free m b0 0 sz) as t; destruct t; try discriminate.
     inv H5; inv H4; simpl in *.
     destruct (Mem.load_loadbytes _ _ _ _ _ Heqp) as [bytes1 [Bytes1 LD1]].
@@ -1297,50 +1365,37 @@ induction 1; intros; try contradiction.
     econstructor. trivial.
     econstructor. split. simpl. rewrite <- Heqt; trivial.
     econstructor.
-(*+ (*builtin*)
-  destruct ef; simpl in *; try solve [elim H4; trivial].
-  - inv H7.
-    destruct (eval_builtin_args_ev_elim_strong _ _ _ _ _ _ _ H6) as [EV EVS].
-    eapply ev_elim_app. eassumption.
-    (*EFexternal helpers don't change memory - should follow from HFD*)
-  - inv H7.
-    destruct (eval_builtin_args_ev_elim_strong _ _ _ _ _ _ _ H6) as [EV EVS].
-    eapply ev_elim_app. eassumption.
-    (*EFbuiltin helpers don't change memory - should follow from HFD*)
-  - (*malloc*)
-    inv H3; inv H7. rewrite H8 in ALLOC. inv ALLOC.
-    destruct (eval_builtin_args_ev_elim_strong _ _ _ _ _ _ _ H6) as [EV EVS].
-    apply Mem.store_storebytes in H9.
-    eapply ev_elim_app. eassumption.
++ (*builtin*)
+  destruct (eval_builtin_args_ev_elim_strong _ _ _ _ _ _ _ H5) as [EV EVS].
+  eapply ev_elim_app. eassumption.
+  inversion H6; subst ef.
+  - inv H3.
+    rewrite Vptrofs_inj with (o2 := n) in H7 by congruence.
+    rewrite H7 in ALLOC. inv ALLOC.
+    apply Mem.store_storebytes in H11.
+    replace (Vptrofs sz) with (Vptrofs n) in H11 by congruence.
     econstructor. split. eassumption.
     econstructor. split. eassumption. constructor.
   - (*free*)
-    inv H3; inv H7.
-    destruct (Mem.load_loadbytes _ _ _ _ _ H8) as [bytes1 [LB1 SZ1]].
-    rewrite LB1 in LB; inv LB. rewrite <- SZ1 in SZ; inv SZ.
-    rewrite H10 in FR; inv FR.
-    destruct (eval_builtin_args_ev_elim_strong _ _ _ _ _ _ _ H6) as [EV EVS].
-    eapply ev_elim_app. eassumption.
+    inv H3.
+    inv H13.
+    destruct (Mem.load_loadbytes _ _ _ _ _ H7) as [bytes1 [LB1 SZ1]].
+    rewrite LB1 in LB; inv LB. rewrite <- SZ1 in SZ.
+    rewrite (Vptrofs_inj _ _ SZ) in *.
+    rewrite H12 in FR; inv FR.
     econstructor. eassumption.
-    econstructor. split. simpl. rewrite H10. reflexivity. constructor.
+    econstructor. split. simpl. rewrite H12. reflexivity. constructor.
   - (*memcpy*)
-    inv H3; inv H7. rewrite LB in H14; inv H14. rewrite ST in H15; inv H15.
-    destruct (eval_builtin_args_ev_elim_strong _ _ _ _ _ _ _ H6) as [EV EVS].
-    eapply ev_elim_app. eassumption.
+    inv H3. inv H18. rewrite LB in H16; inv H16. rewrite ST in H17; inv H17.
     econstructor. eassumption.
-    econstructor. split. eassumption. constructor.*)
-+ eapply extcall_arguments_ev_aux_elim; eassumption.
-(*+ inv H1.
-  destruct callee; simpl in *; try solve [contradiction].
-  - inv H3. (*EFexternal helpers don't change memory - should follow from HFD*)
-  - inv H3. (*EFbuiltin helpers don't change memory - should follow from HFD*)*)
-+ (*loadframe*)
-    eexists. split. eassumption.
-    destruct (store_args_ev_elim _ _ _ _ _ _ H1) as [TT [HTT EV]].
-    unfold store_args_events in H2. rewrite H2 in HTT. inv HTT. trivial.
-Qed. (*due to extcall and builtins -- should all follow from HFD*)
+    econstructor. split. eassumption. constructor.
+  - subst.
+    simpl in *.
+    admit. (* need to know that builtin externals don't change memory *)
+  - (* ditto *) admit.
+Admitted. (*due to extcall and builtins -- should all follow from HFD*)
 
-Lemma store_args_rec_transfer stk m2 mm': forall args tys m1 n
+(*Lemma store_args_rec_transfer stk m2 mm': forall args tys m1 n
  (STARGS: store_args_rec m1 stk n args tys = Some m2) TT
  (STARGSEV: store_args_ev_rec stk n args tys = Some TT) x
  (EV: ev_elim x TT mm'), store_args_rec x stk n args tys = Some mm'.
@@ -1410,7 +1465,7 @@ Proof.
     specialize (IHargs _ _ _ H0 _ Heqp _ EV).
     unfold store_stack; simpl. rewrite Int.add_zero_l in *.
     erewrite Mem.storebytes_store; eassumption.
-Qed.
+Qed.*)
 
 Lemma asm_ev_elim_strong g: forall c m T c' m' (Estep: asm_ev_step g c m T c' m'),
       ev_elim m T m' /\ (forall mm mm', ev_elim mm T mm' -> exists cc', asm_ev_step g c mm T cc' mm').
@@ -1419,8 +1474,8 @@ induction 1; intros; try contradiction.
 + destruct i; inv H2; inv H3; try solve [split;
         first [eexists; split; reflexivity |
                intros mm mm' EV'; inv EV'; destruct H2 as [FL EV']; inv EV'; inv FL;
-                 eexists; econstructor; try eassumption; reflexivity]].
-  - (*Pmov_rm*)
+                 eexists (State _ m1); econstructor; try eassumption; reflexivity]].
+  - (*Pmovl_rm*)
     unfold exec_load in H5.
     remember (Mem.loadv Mint32 m (eval_addrmode g a rs)) as p.
     destruct p; try discriminate; symmetry in Heqp.
@@ -1435,9 +1490,38 @@ induction 1; intros; try contradiction.
       eexists; econstructor; try eassumption; simpl.
       ++ unfold exec_load. rewrite <- Heqq; simpl. erewrite (Mem.loadbytes_load); trivial; eassumption.
       ++ rewrite <- Heqq, H2; reflexivity.
-  - (*Pmov_mr*)
+  - (*Pmovq_rm*)
+    unfold exec_load in H5.
+    remember (Mem.loadv Mint64 m (eval_addrmode g a rs)) as p.
+    destruct p; try discriminate; symmetry in Heqp.
+    remember (eval_addrmode g a rs) as q.
+    destruct q; try discriminate.
+    destruct (Mem.load_loadbytes _ _ _ _ _ Heqp) as [bytes [LB V]]; simpl in LB.
+    rewrite LB in H4; inv H4. inv H5.
+    split.
+    * constructor; simpl; trivial.
+    * intros mm mm' EV'; inv EV'. inv H3.
+      destruct (Mem.load_valid_access _ _ _ _ _ Heqp) as [_ ALIGN].
+      eexists; econstructor; try eassumption; simpl.
+      ++ unfold exec_load. rewrite <- Heqq; simpl. erewrite (Mem.loadbytes_load); trivial; eassumption.
+      ++ rewrite <- Heqq, H2; reflexivity.
+  - (*Pmovl_mr*)
     unfold exec_store in H5.
     remember (Mem.storev Mint32 m (eval_addrmode g a rs) (rs rs0)) as p.
+    destruct p; try discriminate; symmetry in Heqp.
+    remember (eval_addrmode g a rs) as q.
+    destruct q; try discriminate. inv H5; inv H4.
+    destruct (Mem.store_valid_access_3 _ _ _ _ _ _ Heqp) as [_ ALIGN].
+    apply Mem.store_storebytes in Heqp.
+    split.
+    * econstructor. split; simpl; trivial. eassumption.
+    * intros mm mm' EV'; inv EV'. destruct H2. inv H3.
+      eexists; econstructor; try eassumption; simpl.
+      ++ unfold exec_store. rewrite <- Heqq; simpl. erewrite (Mem.storebytes_store); trivial.
+      ++ rewrite <- Heqq; reflexivity.
+  - (*Pmovq_mr*)
+    unfold exec_store in H5.
+    remember (Mem.storev Mint64 m (eval_addrmode g a rs) (rs rs0)) as p.
     destruct p; try discriminate; symmetry in Heqp.
     remember (eval_addrmode g a rs) as q.
     destruct q; try discriminate. inv H5; inv H4.
@@ -1651,22 +1735,46 @@ induction 1; intros; try contradiction.
       eexists; econstructor; try eassumption; simpl.
       ++ unfold exec_load. rewrite <- Heqq; simpl; erewrite (Mem.loadbytes_load); trivial; eassumption.
       ++ rewrite <- Heqq, H2; reflexivity.
-  - (*Pdiv*)
-    remember (Val.divu (rs EAX) (rs # EDX <- Vundef r1)) as p; destruct p; inv H5.
-    remember (Val.modu (rs EAX) (rs # EDX <- Vundef r1)) as q; destruct q; inv H3.
+  - (*Pdivl*)
+    destruct (rs RDX) eqn: HD; inv H5.
+    destruct (rs RAX) eqn: HA; inv H3.
+    destruct (rs r1) eqn: Hr; inv H4.
+    destruct (Int.divmodu2 _ _ _) as [[]|] eqn: Hdiv; inv H3.
     split.
     * eexists; simpl; split; reflexivity.
     * intros mm mm' EV'; inv EV'. destruct H2. inv H3. inv H2.
       eexists; econstructor; try eassumption; simpl; trivial.
-      rewrite <- Heqp, <- Heqq; reflexivity.
-  - (*Pidiv*)
-    remember (Val.divs (rs EAX) (rs # EDX <- Vundef r1)) as p; destruct p; inv H5.
-    remember ( Val.mods (rs EAX) (rs # EDX <- Vundef r1)) as q; destruct q; inv H3.
+      rewrite HD, HA, Hr, Hdiv; reflexivity.
+  - (*Pdivq*)
+    destruct (rs RDX) eqn: HD; inv H5.
+    destruct (rs RAX) eqn: HA; inv H3.
+    destruct (rs r1) eqn: Hr; inv H4.
+    destruct (Int64.divmodu2 _ _ _) as [[]|] eqn: Hdiv; inv H3.
     split.
     * eexists; simpl; split; reflexivity.
     * intros mm mm' EV'; inv EV'. destruct H2. inv H3. inv H2.
       eexists; econstructor; try eassumption; simpl; trivial.
-      rewrite <- Heqp, <- Heqq; reflexivity.
+      rewrite HD, HA, Hr, Hdiv; reflexivity.
+  - (*Pidivl*)
+    destruct (rs RDX) eqn: HD; inv H5.
+    destruct (rs RAX) eqn: HA; inv H3.
+    destruct (rs r1) eqn: Hr; inv H4.
+    destruct (Int.divmods2 _ _ _) as [[]|] eqn: Hdiv; inv H3.
+    split.
+    * eexists; simpl; split; reflexivity.
+    * intros mm mm' EV'; inv EV'. destruct H2. inv H3. inv H2.
+      eexists; econstructor; try eassumption; simpl; trivial.
+      rewrite HD, HA, Hr, Hdiv; reflexivity.
+  - (*Pidivq*)
+    destruct (rs RDX) eqn: HD; inv H5.
+    destruct (rs RAX) eqn: HA; inv H3.
+    destruct (rs r1) eqn: Hr; inv H4.
+    destruct (Int64.divmods2 _ _ _) as [[]|] eqn: Hdiv; inv H3.
+    split.
+    * eexists; simpl; split; reflexivity.
+    * intros mm mm' EV'; inv EV'. destruct H2. inv H3. inv H2.
+      eexists; econstructor; try eassumption; simpl; trivial.
+      rewrite HD, HA, Hr, Hdiv; reflexivity.
   - (*Pcmov*)
     remember (eval_testcond c rs) as p; destruct p; inv H5.
     * destruct b0; inv H3.
@@ -1725,16 +1833,16 @@ induction 1; intros; try contradiction.
   - (*Pjmptbl*)
     remember (rs r) as p; destruct p; inv H5.
     remember (list_nth_z tbl (Int.unsigned i)) as q; destruct q; inv H3.
-    unfold goto_label in H4. rewrite H in *.
+    unfold goto_label in H4. rewrite !Pregmap.gso, H in H4 by discriminate.
     remember (label_pos l 0 (fn_code f)) as w; destruct w; inv H4.
     split.
       * econstructor. split. reflexivity. constructor.
       * intros mm mm' EV'; inv EV'. destruct H2. inv H3. inv H2.
         eexists; econstructor; try eassumption; simpl; try rewrite <- Heqp, <- Heqq; trivial.
-        unfold goto_label. rewrite <- Heqw, H; reflexivity.
+        unfold goto_label. rewrite <- Heqw, !Pregmap.gso, H by discriminate; reflexivity.
   - (*Pmov_rm_a*)
     unfold exec_load in H5.
-    remember (Mem.loadv Many32 m (eval_addrmode g a rs)) as p.
+    remember (Mem.loadv _ m (eval_addrmode g a rs)) as p.
     destruct p; try discriminate; symmetry in Heqp.
     remember (eval_addrmode g a rs) as q.
     destruct q; try discriminate.
@@ -1749,7 +1857,7 @@ induction 1; intros; try contradiction.
       ++ rewrite <- Heqq, H2; reflexivity.
   - (*Pmov_mr_a*)
     unfold exec_store in H5.
-    remember (Mem.storev Many32 m (eval_addrmode g a rs) (rs rs0)) as p.
+    remember (Mem.storev _ m (eval_addrmode g a rs) (rs rs0)) as p.
     destruct p; try discriminate; symmetry in Heqp.
     remember (eval_addrmode g a rs) as q.
     destruct q; try discriminate. inv H5; inv H4.
@@ -1791,33 +1899,33 @@ induction 1; intros; try contradiction.
       ++ unfold exec_store. rewrite <- Heqq; simpl. erewrite (Mem.storebytes_store); trivial.
       ++ rewrite <- Heqq; reflexivity.
   - (*Pallocframe*)
-    remember (Mem.alloc m 0 sz) as a; symmetry in Heqa; destruct a as [m1 stk].
-    remember (Mem.store Mint32 m1 stk
-         (Int.unsigned (Int.add Int.zero ofs_link))
-         (rs ESP)) as p.
+    remember (Mem.alloc m 0 sz) as a; symmetry in Heqa; destruct a as [ma stk].
+    remember (Mem.store Mptr ma stk
+         (Ptrofs.unsigned (Ptrofs.add Ptrofs.zero ofs_link))
+         (rs RSP)) as p.
     destruct p; try discriminate; symmetry in Heqp.
-    remember (Mem.store Mint32 m0 stk (Int.unsigned (Int.add Int.zero ofs_ra))
+    remember (Mem.store Mptr m0 stk (Ptrofs.unsigned (Ptrofs.add Ptrofs.zero ofs_ra))
          (rs RA)) as q.
     destruct q; try discriminate; symmetry in Heqq. inv H5; inv H4.
     destruct (Mem.store_valid_access_3 _ _ _ _ _ _ Heqp) as [_ ALIGNp].
     destruct (Mem.store_valid_access_3 _ _ _ _ _ _ Heqq) as [_ ALIGNq].
     apply Mem.store_storebytes in Heqp.
     apply Mem.store_storebytes in Heqq.
-    rewrite Int.add_zero_l in *.
+    rewrite Ptrofs.add_zero_l in *.
     split.
     * econstructor. split. eassumption.
       econstructor. split. eassumption.
       econstructor. split. eassumption.
       econstructor.
     * intros mm mm' EV'; inv EV'. destruct H2 as [ALLOC EV]. inv EV. inv H2. inv H4. destruct H2. inv H4.
-      eexists; econstructor; try eassumption; simpl; repeat rewrite Int.add_zero_l; rewrite ALLOC;
+      eexists; econstructor; try eassumption; simpl; repeat rewrite Ptrofs.add_zero_l; rewrite ALLOC;
       repeat erewrite Mem.storebytes_store; try eassumption; reflexivity.
   - (*Pfreeframe*)
-    remember (Mem.loadv Mint32 m (Val.add (rs ESP) (Vint ofs_ra))) as p.
+    remember (Mem.loadv Mptr m (Val.offset_ptr (rs RSP) ofs_ra)) as p.
     destruct p; try discriminate; symmetry in Heqp.
-    remember (Mem.loadv Mint32 m (Val.add (rs ESP) (Vint ofs_link))) as q.
+    remember (Mem.loadv Mptr m (Val.offset_ptr (rs RSP) ofs_link)) as q.
     destruct q; try discriminate; symmetry in Heqq.
-    remember (rs ESP) as w; destruct w; try discriminate.
+    remember (rs RSP) as w; destruct w; try discriminate.
     remember (Mem.free m b0 0 sz) as t; destruct t; try discriminate.
     inv H5; inv H4.
     destruct (Mem.load_loadbytes _ _ _ _ _  Heqp) as [bytes1 [Bytes1 LD1]].
@@ -1830,49 +1938,25 @@ induction 1; intros; try contradiction.
       split. simpl. rewrite <- Heqt; trivial. econstructor.
     * intros mm mm' EV'. inv EV'. inv H3. inv H5. destruct H3. inv H5. simpl in H3.
       remember (Mem.free mm b0 0 sz) as d; destruct d; try discriminate. inv H3.
-      exploit (Mem.loadbytes_load Mint32). apply H2. assumption.
-      exploit (Mem.loadbytes_load Mint32). apply H4. assumption.
+      exploit (Mem.loadbytes_load Mptr). apply H2. assumption.
+      exploit (Mem.loadbytes_load Mptr). apply H4. assumption.
       eexists; econstructor; try eassumption.
       ++ simpl. rewrite <- Heqw; simpl. rewrite H3, H5, <- Heqd. reflexivity.
       ++ simpl. rewrite <- Heqw; simpl. rewrite H3, H5, <- Heqd. rewrite H2, H4. reflexivity.
-(* + (*builtin*)
-  destruct ef; simpl in *; try solve [elim H4; trivial].
-  - inv H7.
-    destruct (eval_builtin_args_ev_elim_strong _ _ _ _ _ _ _ H6) as [EV EVS].
-    split.
-    * eapply ev_elim_app. eassumption.
-      (*EFexternal helpers don't change memory - should follow from HFD*)
-    * intros mm mm' MM. rewrite app_nil_r in MM.
-      destruct (EVS _ _ MM); subst mm'.
-      destruct (I64Helpers.is_I64_helperS_dec name sg). 2: elim H4; trivial.
-      (*helpers don't access memory -- with stengthened HFD, proof will essesntially be like this:
-      eexists. eapply asm_ev_step_builtin; try eassumption. simpl; trivial.
-        eapply eval_builtin_args_ev_eval_builtin_args; eassumption.
-        2: reflexivity.
-        2: constructor; trivial. *)
-  - inv H7.
-    destruct (eval_builtin_args_ev_elim_strong _ _ _ _ _ _ _ H6) as [EV EVS].
-    split.
-    * eapply ev_elim_app. eassumption.
-      (*EFbuiltin helpers don't change memory - should follow from HFD*)
-    * intros mm mm' MM. rewrite app_nil_r in MM.
-      destruct (EVS _ _ MM); subst mm'.
-      destruct (is_I64_builtinS_dec name sg). 2: elim H4; trivial.
-       (*helpers don't access memory -- with stengthened HFD, proof will essesntially be like this:
-      eexists. eapply asm_ev_step_builtin; try eassumption. simpl; trivial.
-        eapply eval_builtin_args_ev_eval_builtin_args; eassumption.
-        2: reflexivity.
-        2: constructor; trivial. *)
++ (*builtin*)
+  destruct (eval_builtin_args_ev_elim_strong _ _ _ _ _ _ _ H5) as [EV EVS].
+  inversion H6; subst ef.
   - (*malloc*)
-    inv H3; inv H7. rewrite H8 in ALLOC. inv ALLOC.
-    destruct (eval_builtin_args_ev_elim_strong _ _ _ _ _ _ _ H6) as [EV EVS].
-    apply Mem.store_storebytes in H9.
+    inv H3. rewrite Vptrofs_inj with (o2 := n) in H7 by congruence.
+    rewrite H7 in ALLOC. inv ALLOC.
+    replace (Vptrofs sz) with (Vptrofs n) in H11 by congruence.
+    apply Mem.store_storebytes in H11.
     split.
     * eapply ev_elim_app. eassumption.
       econstructor. split. eassumption.
       econstructor. split. eassumption. constructor.
     * intros mm mm' MM. apply ev_elim_split in MM; destruct MM as [mm1 [EV1 EV2]].
-      inv EV2. destruct H3. inv H5. destruct H7. inv H7.
+      inv EV2. destruct H3. inv H4. destruct H8. inv H8.
       rename x into mm2. rename x0 into mm3.
       specialize (EVS _ _ EV1); destruct EVS; subst mm1.
       eexists. eapply asm_ev_step_builtin; try eassumption; simpl; trivial.
@@ -1880,43 +1964,67 @@ induction 1; intros; try contradiction.
       ++ econstructor. eassumption. erewrite Mem.storebytes_store; try reflexivity; eassumption.
       ++ econstructor; try eassumption.
   - (*free*)
-    inv H3; inv H7.
-    destruct (Mem.load_loadbytes _ _ _ _ _ H8) as [bytes1 [LB1 SZ1]].
-    rewrite LB1 in LB; inv LB. rewrite <- SZ1 in SZ; inv SZ.
-    rewrite H10 in FR; inv FR.
-    destruct (eval_builtin_args_ev_elim_strong _ _ _ _ _ _ _ H6) as [EV EVS].
+    inv H3. inv H13.
+    destruct (Mem.load_loadbytes _ _ _ _ _ H7) as [bytes1 [LB1 SZ1]].
+    rewrite LB1 in LB; inv LB. rewrite <- SZ1 in SZ. rewrite (Vptrofs_inj _ _ SZ) in *.
+    rewrite H12 in FR; inv FR.
     split.
     * eapply ev_elim_app. eassumption.
       econstructor. eassumption.
-      econstructor. split. simpl. rewrite H10. reflexivity. constructor.
+      econstructor. split. simpl. rewrite H12. reflexivity. constructor.
     * intros mm mm' MM. apply ev_elim_split in MM; destruct MM as [mm1 [EV1 EV2]].
-      inv EV2. inv H5. destruct H7. inv H7.
+      inv EV2. inv H4. destruct H8. inv H8.
       rename x into mm2.
       specialize (EVS _ _ EV1); destruct EVS; subst mm1.
-      simpl in H5.
-      remember (Mem.free mm b0 (Int.unsigned lo - 4) (Int.unsigned lo + Int.unsigned sz)) as d.
-      destruct d; inv H5; symmetry in Heqd.
+      simpl in H4.
+      remember (Mem.free mm b0 (Ptrofs.unsigned lo - size_chunk Mptr) (Ptrofs.unsigned lo + Ptrofs.unsigned sz0)) as d.
+      destruct d; inv H4; symmetry in Heqd.
       eexists. eapply asm_ev_step_builtin; try eassumption; simpl; trivial.
       ++ eapply eval_builtin_args_ev_eval_builtin_args; eassumption.
       ++ econstructor; try eassumption.
          rewrite SZ1. apply Mem.loadbytes_load; assumption.
       ++ econstructor; eassumption.
   - (*memcpy*)
-    inv H3; inv H7. rewrite LB in H14; inv H14. rewrite ST in H15; inv H15.
-    destruct (eval_builtin_args_ev_elim_strong _ _ _ _ _ _ _ H6) as [EV EVS].
+    inv H3. inv H18. rewrite LB in H16; inv H16. rewrite ST in H17; inv H17.
     split.
     * eapply ev_elim_app. eassumption.
       econstructor. eassumption.
       econstructor. split. eassumption. constructor.
     * intros mm mm' MM. apply ev_elim_split in MM; destruct MM as [mm1 [EV1 EV2]].
-      inv EV2. inv H5. destruct H7. inv H7.
+      inv EV2. inv H4. destruct H8. inv H8.
       rename x into mm2.
       specialize (EVS _ _ EV1); destruct EVS; subst mm1.
       eexists. eapply asm_ev_step_builtin; try eassumption; simpl; trivial.
       ++ eapply eval_builtin_args_ev_eval_builtin_args; eassumption.
       ++ econstructor; try eassumption.
-      ++ econstructor; eassumption.*)
-+ (*Step-to-external*)
+      ++ econstructor; eassumption.
+  - subst.
+    split.
+    * eapply ev_elim_app. eassumption.
+      (*EFexternal helpers don't change memory - should follow from HFD*)
+      admit.
+    * intros mm mm' MM. rewrite app_nil_r in MM.
+      destruct (EVS _ _ MM); subst mm'.
+      (*helpers don't access memory -- with stengthened HFD, proof will essesntially be like this:
+      eexists. eapply asm_ev_step_builtin; try eassumption. simpl; trivial.
+        eapply eval_builtin_args_ev_eval_builtin_args; eassumption.
+        2: reflexivity.
+        2: constructor; trivial. *)
+      admit.
+  - subst.
+    split.
+    * eapply ev_elim_app. eassumption.
+      (*EFbuiltin helpers don't change memory - should follow from HFD*)
+      admit.
+    * intros mm mm' MM. rewrite app_nil_r in MM.
+      destruct (EVS _ _ MM); subst mm'.
+       (*helpers don't access memory -- with stengthened HFD, proof will essesntially be like this:
+      eexists. eapply asm_ev_step_builtin; try eassumption. simpl; trivial.
+        eapply eval_builtin_args_ev_eval_builtin_args; eassumption.
+        2: reflexivity.
+        2: constructor; trivial. *)
+      admit.
+(*+ (*Step-to-external*)
   exploit extcall_arguments_ev_aux_elim_strong. apply H2. intros [EV HEV].
   split; trivial; intros.
   destruct (HEV _ _ H3); subst.
@@ -1932,16 +2040,15 @@ induction 1; intros; try contradiction.
    * econstructor. split; eassumption.
    * intros mm mm' EV'. inv EV'. destruct H3.
      exploit store_args_rec_transfer. eassumption. eassumption. eassumption. intros SAR.
-     eexists. econstructor; try eassumption.
-Qed. (*due to extcall and builtins*)
+     eexists. econstructor; try eassumption.*)
+Admitted. (*due to extcall and builtins*)
 
-Program Definition Asm_EvSem : @EvSem genv state.
-Proof.
-eapply Build_EvSem with (msem := Asm_mem_sem (*hf*)) (ev_step:=asm_ev_step).
-+ intros. eapply asm_ev_ax1; try eassumption. (*helper_functions declared*)
-+ eapply asm_ev_ax2; eassumption.
+Definition Asm_EvSem (prog : program) : @EvSem genv state.
+eapply Build_EvSem with (msem := Asm_mem_sem prog (*hf*)) (ev_step:=asm_ev_step).
++ intros. assert (g = Genv.globalenv prog) by admit; subst. eapply asm_ev_ax1; try eassumption. (*helper_functions declared*)
++ intros. assert (g = Genv.globalenv prog) by admit; subst. eapply asm_ev_ax2; eassumption.
 + eapply asm_ev_fun; eassumption.
 + eapply asm_ev_elim_strong; eassumption.
-Defined. (*helper_functions declared*)
+Admitted. (*helper_functions declared*)
 
 End ASM_EV.
